ttcan: wip specification for triggers

example/ttcan/Network.TTCan.Impl.Util.fst
@@ -2,6 +2,7 @@ module Network.TTCan.Impl.Util
 
 module S       = Pipit.Sugar.Shallow
 module U64     = Network.TTCan.Prim.U64
+module S32R    = Network.TTCan.Prim.S32R
 
 open Pipit.Sugar.Shallow.Tactics.Lift
 open Network.TTCan.Types
@@ -27,6 +28,20 @@ let falling_edge
     : stream bool =
   not v && (false `fby` v)
 
+(* Check whether the value stream `v` only changes when clock `k` is true.
+  (That is, if v is sampled on k)
+
+  This is related to `edge`, in that:
+  > is_sampled_on v (edge v)
+  always holds
+
+  *)
+let is_sampled_on
+  (#a: eqtype) {| S.has_stream a |}
+  (v: stream a)
+  (k: stream bool)
+    : stream bool =
+  true ->^ (v = pre v || k)
 
 (* Resettable latch.
   Named arguments would be nice. It's easy to confuse the set/reset so we
@@ -49,9 +64,32 @@ let latch (args: stream latch_args): stream bool =
     else (false `fby` latch)
   in latch
 
+(**** Time utilities ***)
 
-let time_ascending (local_time: stream ntu): stream bool =
+(* The driver performs a "tick" at least every ttcan_exec_period ntus.
+  The time must be increasing and increase by at most ttcan_exec_period.
+  The initial value of the time does not necessarily need to be 0.
+*)
+let local_time_valid (cfg: config) (local_time: stream ntu): stream bool =
   let open U64 in
-  0uL `fby` local_time < local_time
+  let prev = pre local_time in
+  let next = prev + S32R.s32r_to_u64 cfg.triggers.ttcan_exec_period in
+  true ->^ (prev < local_time && local_time <= next)
 
-%splice[] (autolift_binds [`%edge; `%rising_edge; `%falling_edge; `%latch; `%time_ascending])
+(* The cycle time is the time relative to the start of the current basic cycle.
+  Whenever the reference clock indicates the start of a new basic cycle, the
+  cycle time resets. We allow a period's slack time between the actual reset and
+  the reference clock, as the driver might not be called immediately.
+*)
+let cycle_time_valid (cfg: config) (ref_ck: stream bool) (cycle_time: stream ntu): stream bool =
+  let open U64 in
+  let ttcan_exec_period = S32R.s32r_to_u64 cfg.triggers.ttcan_exec_period in
+  let prev = pre cycle_time in
+  let next = prev + ttcan_exec_period in
+  // Reset on first step and on reference clock
+  if true ->^ ref_ck
+  then cycle_time < ttcan_exec_period
+  else prev < cycle_time && cycle_time <= next
+
+
+%splice[] (autolift_binds [`%edge; `%rising_edge; `%falling_edge; `%is_sampled_on; `%latch; `%local_time_valid; `%cycle_time_valid])
