example/ttcan/Network.TTCan.Types.Base.fst
@@ -1,0 +1,77 @@
+(* Base type definitions *)
+module Network.TTCan.Types.Base
+
+module U64        = Network.TTCan.Prim.U64
+module Subrange   = Network.TTCan.Prim.S32R
+
+module List       = FStar.List.Tot
+
+type mode =
+  | Mode_Configure | Mode_Running
+
+type sync_mode =
+  | Sync_Off | Synchronising | In_Schedule // not supported: In_Gap
+type master_mode =
+  | Master_Off | Follower | Current_Master | Backup_Master
+type error_severity =
+  | S0_No_Error | S1_Warning | S2_Error | S3_Severe
+
+type tx_status =
+  | Tx_None | Tx_Ok | Tx_Lost_Arbitration | Tx_Error
+type bus_status =
+  | Bus_Idle | Bus_Busy | Bus_Bad | Bus_Off
+
+type trigger_type =
+  | Tx_Trigger | Rx_Trigger | Tx_Ref_Trigger | Watch_Trigger
+
+(* Network time unit: time in terms of CAN-bitrate clock. The spec specifies a 16-bit local time that overflows regularly, but for now we'll use 64-bit to avoid worrying about overflow. *)
+type ntu = U64.t
+
+// configuration values can be statically limited to 16-bits
+type ntu_config = Subrange.t { min = 0; max = 65535 } // U16.t
+
+(* @7.4.3 Ref_Trigger_Offset may only take values between -127 [sic] and 127. *)
+type ref_offset    = Subrange.t { min = -127; max = 127 }
+type master_index  = Subrange.t { min = 0; max = 7 }
+type cycle_index   = Subrange.t { min = 0; max = 63 }
+// power-of-two denoting how often to repeat
+type repeat_factor = Subrange.t { min = 0; max = 6 }
+
+type ref_message = {
+  sof:         ntu;
+  master:      master_index;
+  cycle_index: cycle_index;
+  // Next_Is_Gap not supported
+}
+
+type message_status_counter = Subrange.t { min = 0; max = 7 }
+
+let max_can_buffer_id = 63
+type can_buffer_id = Subrange.t { min = 0; max = max_can_buffer_id }
+
+type trigger = {
+  trigger_type:  trigger_type;
+  time_mark:     ntu_config;
+  cycle_offset:  cycle_index;
+  repeat_factor: repeat_factor;
+  message_index: can_buffer_id;
+}
+
+type fault_bits = {
+  scheduling_error_1:    bool;
+  tx_underflow:          bool;
+  scheduling_error_2:    bool;
+  tx_overflow:           bool;
+  can_bus_off:           bool;
+  watch_trigger_reached: bool;
+}
+
+let init_watch_trigger_time: ntu_config = Subrange.s32r 65535
+
+(* The M_TTCAN implementation supports at most 64 triggers, so we apply the same limit. *)
+let max_trigger_index = 63
+let max_trigger_count = max_trigger_index + 1
+type trigger_index = Subrange.t { min = 0; max = max_trigger_index }
+type trigger_count = Subrange.t { min = 0; max = max_trigger_count }
+
+type tx_enable_window = Subrange.t { min = 1; max = 16 } // spec says upper limit is 16 - why 16?
