example/ttcan/Network.TTCan.Types.Triggers.fst
@@ -1,0 +1,171 @@
+module Network.TTCan.Types.Triggers
+
+open Network.TTCan.Types.Base
+
+module U64        = Network.TTCan.Prim.U64
+module Subrange   = Network.TTCan.Prim.S32R
+
+module List       = FStar.List.Tot
+
+module UInt8      = FStar.UInt8
+module UInt64     = FStar.UInt64
+module Cast       = FStar.Int.Cast
+
+open FStar.Mul
+
+(* We assume a total, safe indexing function for triggers.
+  The actual implementation will likely be backed by a read-only array. Since
+  we only support at most 64 triggers, it doesn't really hurt to allocate space
+  for all 64 of them.
+*)
+type trigger_index_fun = trigger_index -> trigger
+
+(***** Non-streaming helper functions ****)
+let trigger_check_enabled (cycle_index: cycle_index) (trigger: trigger): bool =
+  let mask    = Subrange.pow2_minus_one trigger.repeat_factor in
+  let mask8   = Subrange.s32r_to_u8 mask in
+  let index8  = Subrange.s32r_to_u8 cycle_index in
+  let offset8 = Subrange.s32r_to_u8 trigger.cycle_offset in
+  UInt8.logand mask8 index8 = offset8
+
+let trigger_tx_ref_expiry (tx_enable_window: tx_enable_window) (ix: trigger_index) (trigger: trigger): ntu =
+  let open UInt64 in
+  let tm = Subrange.s32r_to_u64 trigger.time_mark in
+  tm +^ Subrange.s32r_to_u64 tx_enable_window
+
+let trigger_offset (ref_trigger_offset: ref_offset) (tr: trigger): trigger =
+  let time_mark =
+    match tr.trigger_type with
+    | Tx_Ref_Trigger ->
+      // use saturating addition to clamp to [0,65535]
+      Subrange.add_sat tr.time_mark ref_trigger_offset
+    | _ ->
+      tr.time_mark
+  in
+  { tr with time_mark }
+
+(***** Requirements on trigger array ****)
+
+(* Time-marks are sorted *)
+let time_mark_sorted_all (trigger_read: trigger_index_fun): prop =
+  forall (i: trigger_index).
+    Subrange.v (trigger_read                   i).time_mark <=
+    Subrange.v (trigger_read (Subrange.inc_sat i)).time_mark
+
+(* Adequate time gap between triggers enabled on same cycle *)
+let adequate_spacing (trigger_read: trigger_index_fun) (ttcan_exec_period: ntu_config) (c: cycle_index) (i j: trigger_index): prop =
+  Subrange.v i <= Subrange.v j                             ==>
+  trigger_check_enabled c (trigger_read i) ==>
+  trigger_check_enabled c (trigger_read j) ==>
+  (Subrange.v (trigger_read i).time_mark - Subrange.v (trigger_read j).time_mark) >= (Subrange.v j - Subrange.v i) * Subrange.v ttcan_exec_period
+
+let adequate_spacing_all (trigger_read: trigger_index_fun) (ttcan_exec_period: ntu_config): prop =
+  forall (c: cycle_index). forall (i j: trigger_index).
+    adequate_spacing trigger_read ttcan_exec_period c i j
+
+(* Adequate time gap from start of array to trigger *)
+let time_mark_reachable_all (trigger_read: trigger_index_fun) (ttcan_exec_period: ntu_config): prop =
+  forall (i: trigger_index).
+    Subrange.v i * Subrange.v ttcan_exec_period <= Subrange.v (trigger_read i).time_mark
+
+(* Trigger configuration: the array as an index function, the period of
+  execution frequency (eg once per 10µs), as well as the proofs that the array
+  represents a valid schedule. *)
+noeq
+type triggers = {
+  trigger_read: trigger_index_fun;
+  ttcan_exec_period: ntu_config;
+
+  time_mark_sorted_all: squash (time_mark_sorted_all trigger_read);
+  adequate_spacing_all: squash (adequate_spacing_all trigger_read ttcan_exec_period);
+  time_mark_reachable_all: squash (time_mark_reachable_all trigger_read ttcan_exec_period);
+}
+
+(* Compute the index of the next active trigger (specification only).
+  This should be equivalent to the index with the minimum start time of all
+  future enabled triggers. If no such triggers exist, it returns
+  max_trigger_count (one past the end of the array).
+
+  Note Specification Only
+  -----------------------
+  This function must not be called as executable code, as it would have the
+  wrong complexity (linear in the number of triggers, rather than constant).
+  We mark it as noextract so it can't be extracted. Really it should be ghost,
+  but Pipit doesn't support ghost code yet.
+  *)
+noextract
+let rec active_next_after_index (trigger_read: trigger_index_fun) (cycle_index: cycle_index) (time: nat) (index: nat { 0 <= index /\ index <= max_trigger_count })
+  : Tot
+    (n: nat { index <= n /\ n <= max_trigger_count })
+    (decreases (max_trigger_count - index)) =
+  if index >= max_trigger_count
+  then max_trigger_count
+  else
+    let tr = trigger_read (Subrange.s32r index) in
+    if Subrange.v tr.time_mark > time && trigger_check_enabled cycle_index tr
+    then index
+    else active_next_after_index trigger_read cycle_index time (index + 1)
+
+(* Index of the next active trigger (specification only) *)
+noextract
+let active_next_after (trigger_read: trigger_index_fun) (cycle_index: cycle_index) (time: nat)
+  : (n: nat { 0 <= n /\ n <= max_trigger_count }) =
+  active_next_after_index trigger_read cycle_index time 0
+
+(* Compute the index of the most-recent active trigger (specification only).
+  This should be equivalent to the index with the maximum start time of all
+  triggers whose start time is now or in the past. If no such triggers exist,
+  it returns zero.
+*)
+noextract
+let rec active_now_index (trigger_read: trigger_index_fun) (cycle_index: cycle_index) (time: nat) (index: nat { index < max_trigger_count })
+  : Tot
+    (n: nat { 0 <= n /\ n < max_trigger_count })
+    (decreases index) =
+  if index = 0
+  then 0
+  else
+    let tr = trigger_read (Subrange.s32r index) in
+    if Subrange.v tr.time_mark <= time && trigger_check_enabled cycle_index tr
+    then index
+    else active_now_index trigger_read cycle_index time (index - 1)
+
+(* Index of the most-recent active trigger *)
+noextract
+let active_now (trigger_read: trigger_index_fun) (cycle_index: cycle_index) (time: nat)
+  : (n: nat { 0 <= n /\ n < max_trigger_count }) =
+  active_now_index trigger_read cycle_index time max_trigger_index
+
+
+(* True if trigger will start before the end of this frame, or has already started *)
+noextract
+let trigger_started (triggers: triggers) (cycle_time: nat) (time_mark: nat): bool =
+  time_mark <= cycle_time + Subrange.v triggers.ttcan_exec_period
+
+(* True if trigger starts in this frame *)
+noextract
+let trigger_impending (triggers: triggers) (cycle_time: nat) (time_mark: nat): bool =
+  cycle_time < time_mark && time_mark <= cycle_time + Subrange.v triggers.ttcan_exec_period
+
+
+irreducible
+let lemma_adequate_spacing_next_inc_pattern (triggers: triggers) (c: cycle_index) (time: ntu) (i: trigger_index) = ()
+
+let lemma_adequate_spacing_next_inc
+  (triggers: triggers) (c: cycle_index) (time: ntu) (i: trigger_index)
+  : Lemma
+    (ensures (
+       let n = active_next_after_index triggers.trigger_read c (UInt64.v time) (Subrange.v i) in
+       n < max_trigger_count ==>
+       adequate_spacing triggers.trigger_read triggers.ttcan_exec_period i (Subrange.s32r n) c
+    ))
+    [SMTPat (lemma_adequate_spacing_next_inc_pattern triggers c time i)]
+    = ()
+
+// let trigger_index_invariant (cfg: config) (c: cycle) (now: time) (index: index): bool =
+//   match next cfg.triggers index c with
+//   | None -> true
+//   | Some n -> (cfg.triggers.time_mark n - now) >= (n - index)
+
+// let trigger_fetch_guar (cfg: config) (c: cycle) (index: stream int) (now: stream int): stream bool =
+//   (index < cfg.triggers.size && trigger_enabled cfg index c) ==> trigger_time_mark cfg index >= now
